fairness/fuel_ext.v
@@ -164,5 +164,33 @@ Section LsTmap.
     - apply ls_mapping_tmap_corr. 
     - by rewrite build_LS_ext_spec_tmap.
   Qed.
+  
+  Definition initial_ls_LSI s0 (g: G) :=
+    let f0 := gset_to_gmap (LM.(lm_fl) s0) (M.(live_roles) s0) in
+    let m0 := gset_to_gmap g (M.(live_roles) s0) in
+    LSI s0 m0 f0.
+
+  (* TODO: use Program after changing the definition of LiveState *)
+  Definition initial_ls' (s0: M) (ζ0: G)
+    (f0 := gset_to_gmap (LM.(lm_fl) s0) (M.(live_roles) s0))
+    (tm0 := {[ ζ0 := M.(live_roles) s0 ]}: gmap G (gset (fmrole M)))
+    (* (LSI0: LSI s0 (ls_mapping_impl tm0) f0)  *)
+    (LSI0: initial_ls_LSI s0 ζ0)
+    : LM.(lm_ls).
+    assert (tmap_disj tm0) as DISJ0.
+    { subst tm0. intros ????. repeat setoid_rewrite lookup_singleton_Some.
+      by intros ? [-> <-] [-> <-]. }
+    unshelve eapply (@build_LS_ext  s0 f0 _ tm0 _ _); eauto. 
+    - simpl. intros. apply reflexive_eq. rewrite dom_gset_to_gmap //.
+    - intros. subst tm0. setoid_rewrite lookup_singleton_Some.
+      subst f0. rewrite dom_gset_to_gmap.
+      split.
+      + intros; eauto.
+      + intros (?&?&[-> <-]&?); eauto.
+    - red in LSI0. fold f0 in LSI0.
+      erewrite maps_inverse_match_uniq1 with (m1 := ls_mapping_impl tm0); eauto.
+      { apply ls_mapping_tmap_corr_impl; eauto. }
+      subst tm0. apply maps_inverse_match_exact.
+  Defined. 
 
 End LsTmap.
