fairness/heap_lang/simulation_adequacy_lm.v
@@ -3,38 +3,14 @@ From trillium.fairness Require Import fuel fuel_termination fairness_finiteness 
 From trillium.fairness.heap_lang Require Import lang simulation_adequacy em_lm_heap_lang em_lm.
 
 
-(* TODO: move, change initial_ls definition *)
-Definition initial_ls_pre `{LM: LiveModel G M LSI} s0 (g: G) :=
-  let f0 := gset_to_gmap (LM.(lm_fl) s0) (M.(live_roles) s0) in
-  let m0 := gset_to_gmap g (M.(live_roles) s0) in
-  (m0, f0). 
-
-Definition initial_ls_LSI `{LM: LiveModel G M LSI} s0 (g: G) :=
-  let '(m0, f0) := initial_ls_pre s0 g (LM := LM) in 
-  LSI s0 m0 f0. 
-
-Program Definition initial_ls' `{LM: LiveModel G M LSI} s0 (g: G)
-  (LSI0: initial_ls_LSI s0 g (LM := LM))
-  : LM.(lm_ls)
-  :=
-  let '(m0, f0) := initial_ls_pre s0 g (LM := LM) in
-  {| ls_under := s0;
-    ls_fuel := f0;
-    ls_mapping := m0;
-  |}. 
-  Next Obligation. 
-    simpl. rewrite /initial_ls_pre. intros. inversion Heq_anonymous. subst. 
-    apply reflexive_eq. rewrite dom_gset_to_gmap //.
-  Qed.
-  Next Obligation. 
-    simpl. rewrite /initial_ls_pre. intros. inversion Heq_anonymous. subst. 
-    apply reflexive_eq. rewrite !dom_gset_to_gmap //. 
-  Qed.
-  Next Obligation.
-    simpl. rewrite /initial_ls_pre. intros. inversion Heq_anonymous. subst. 
-    done.
-  Qed. 
-
+(* TODO: move *)
+Lemma initial_ls'_mapping `{LM : LiveModel G M LSI} `{Countable G} s0 g LSI0:
+  ls_mapping (initial_ls' s0 g LSI0 (LM := LM)) = gset_to_gmap g (live_roles M s0).
+Proof.
+  rewrite /initial_ls'. erewrite build_LS_ext_spec_mapping; [reflexivity| ].
+  apply maps_inverse_match_exact. 
+Qed. 
+  
 
 Section adequacy.
 (* Local Hint Resolve tid_step_tp_length_heap: core. *)
@@ -52,7 +28,7 @@ Theorem heap_lang_continued_simulation_fair_termination
   :
   continued_simulation
     (sim_rel_with_user LM ξ)
-    ({tr[trfirst extr]}) ({tr[initial_ls a1 r1 LSI0]}) →
+    ({tr[trfirst extr]}) ({tr[initial_ls' a1 r1 LSI0]}) →
   extrace_fairly_terminating extr.
 Proof.
   apply continued_simulation_fair_termination.
@@ -68,19 +44,19 @@ Let rel_always_holds `{hGS: @heapGS Σ (fair_model_model LM_Fair) (@LM_EM_HL _ _
         s (state_interp) (fun _ => frag_mapping_is {[ 0%nat := ∅ ]} (LM := LM)) e1 σ1 δ1. 
 
 
-(* TODO: should hold by definition after changing LiveState *)
-Lemma initial_ls_tmap τ s (LSI0: initial_ls_LSI s τ):
-  ls_tmap (initial_ls s τ LSI0) (LM := LM) = {[ τ := live_roles M s ]}.
-Proof. Admitted. 
+(* (* TODO: should hold by definition after changing LiveState *) *)
+(* Lemma initial_ls_tmap τ s (LSI0: initial_ls_LSI s τ): *)
+(*   ls_tmap (initial_ls s τ LSI0) (LM := LM) = {[ τ := live_roles M s ]}. *)
+(* Proof. Admitted.  *)
 
 
 Lemma rel_always_holds_lift_LM 
   `{hGS: @heapGS Σ (fair_model_model LM_Fair) (@LM_EM_HL _ _ _ LF')}
   s e1 σ1 s1 ξ
   (LSI0: initial_ls_LSI s1 0):
-  rel_always_holds s ξ e1 σ1 (initial_ls s1 0%nat LSI0) -∗
+  rel_always_holds s ξ e1 σ1 (initial_ls' s1 0%nat LSI0) -∗
   rel_always_holds0 (sim_rel_with_user LM ξ) s state_interp
-    (λ _, frag_mapping_is {[ 0%nat := ∅ ]}) e1 σ1 (initial_ls s1 0%nat LSI0).
+    (λ _, frag_mapping_is {[ 0%nat := ∅ ]}) e1 σ1 (initial_ls' s1 0%nat LSI0).
 Proof.
   iIntros "H".
   iIntros (ex atr c Hvalex Hstartex Hstartatr Hendex Hcontr Hstuck Hequiv) "Hsi Hposts".
@@ -108,15 +84,16 @@ Proof.
     simplify_eq.
     iApply (fupd_mask_weaken ∅); first set_solver. iIntros "_ !>".
     assert (∀ (ρ : fmrole M) (tid : nat),
-               ls_mapping (initial_ls (LM := LM) s1 0%nat LSI0) !! ρ = Some tid →
+               ls_mapping (initial_ls' (LM := LM) s1 0%nat LSI0) !! ρ = Some tid →
                is_Some (([e1], σ1).1 !! tid)) as HA.
-    { simpl. intros ρ tid Hsome. apply lookup_gset_to_gmap_Some in Hsome as [??].
-      simplify_eq. by eexists _. }
+    { simpl. rewrite initial_ls'_mapping. 
+      setoid_rewrite lookup_gset_to_gmap_Some.
+      intros ?? [? <-]. by eexists _. }
     iSplit; last done. iClear "H1".
     iSplit; first done.
     destruct (to_val e1) as [v1|] eqn:Heq.
     + iSplit.
-      { iPureIntro. intros ρ tid Hinit.
+      { iPureIntro. rewrite initial_ls'_mapping. intros ρ tid Hinit.
         simpl in *. apply lookup_gset_to_gmap_Some in Hinit as [_ <-].
         rewrite /from_locale //. }
       iIntros (tid e Hsome Hnoval ρ). destruct tid; last done.
@@ -127,9 +104,11 @@ Proof.
       iDestruct "Hsi" as "(%FR'&Hfuela&Hmapa&HFR&Hmodel&HfrFR)".
       iDestruct (frag_mapping_same 0%nat with "[Hmapa] Hem") as "%H"; [done| ].
       iPureIntro. eapply no_locale_empty; [| done].
-      rewrite initial_ls_tmap. apply maps_inverse_match_exact. 
+      rewrite initial_ls'_mapping. rewrite build_LS_ext_spec_tmap.
+      apply maps_inverse_match_exact. 
     + iSplit; iPureIntro.
-      { simpl. intros ρ tid Hsome. apply lookup_gset_to_gmap_Some in Hsome as [??].
+      { simpl. rewrite initial_ls'_mapping. intros ρ tid Hsome.
+        apply lookup_gset_to_gmap_Some in Hsome as [??].
         simplify_eq. by eexists _. }
       intros tid e Hsome Hval' ρ.
       destruct tid as [|tid]; rewrite /from_locale /= in Hsome; by simplify_eq.
@@ -166,7 +145,7 @@ Definition wp_premise
   `{hPre: @heapGpreS Σ (fair_model_model LM_Fair) (@LM_EM_HL _ _ _ LF')}
   ξ σ1 e1 s1 s FR
   (LSI0: initial_ls_LSI s1 0)
-  (δ0 := initial_ls (LM := LM) s1 0%nat LSI0)
+  (δ0 := initial_ls' (LM := LM) s1 0%nat LSI0)
     := (∀ `{hGS: @heapGS Σ (fair_model_model LM_Fair) (@LM_EM_HL _ _ _ LF')}, 
     ⊢ (|={⊤}=>
        (* ([∗ map] l ↦ v ∈ heap σ1, mapsto l (DfracOwn 1) v) ∗ *)
@@ -180,7 +159,7 @@ Theorem strong_simulation_adequacy Σ
     (ξ : execution_trace heap_lang → finite_trace M (option $ fmrole M) →
          Prop)    
   (LSI0: initial_ls_LSI s1 0)
-  (δ0 := initial_ls (LM := LM) s1 0%nat LSI0)
+  (δ0 := initial_ls' (LM := LM) s1 0%nat LSI0)
   :
   rel_finitary (sim_rel_with_user LM ξ) →
   (∀ `{hGS: @heapGS Σ (fair_model_model LM_Fair) (@LM_EM_HL _ _ _ LF')},
@@ -199,7 +178,9 @@ Proof.
   1,2,4: done.
   { split.
     - red. eauto.
-    - red. split; auto. apply initial_ls_tmap.  } 
+    - red. split.
+      + by rewrite build_LS_ext_spec_st build_LS_ext_spec_fuel.
+      + by rewrite build_LS_ext_spec_tmap build_LS_ext_spec_st. } 
   iIntros (?) "INIT".
   iMod (WP_RAH Hinv) as "WP_RAH".
   iMod ("WP_RAH" with "INIT") as "[WP RAH]".
@@ -209,7 +190,7 @@ Qed.
 
 Theorem simulation_adequacy Σ  `{hPre: @heapGpreS Σ (fair_model_model LM_Fair) (@LM_EM_HL _ _ _ LF')} (s: stuckness) (e1 : expr heap_lang) σ1 (s1: M) FR
   (LSI0: initial_ls_LSI s1 0)
-  (δ0 := initial_ls (LM := LM) s1 0%nat LSI0)
+  (δ0 := initial_ls' (LM := LM) s1 0%nat LSI0)
 :
   (* The model has finite branching *)
   rel_finitary (sim_rel LM) →
@@ -262,7 +243,7 @@ Theorem simulation_adequacy_inftraces Σ
        (fair_model_model LM_Fair)
        (sim_rel LM))
     (trace_singleton ([e1], σ1))
-    (trace_singleton (initial_ls (LM := LM) s1 0%nat LSI0))
+    (trace_singleton (initial_ls' (LM := LM) s1 0%nat LSI0))
     iex
     iatr.
 Proof.
@@ -301,14 +282,14 @@ Proof.
            (fair_model_model LM_Fair)
            (sim_rel LM))
         (trace_singleton ([e1], (trfirst extr).2))
-        (trace_singleton (initial_ls (LM := LM) s1 0%nat LSI0))
+        (trace_singleton (initial_ls' (LM := LM) s1 0%nat LSI0))
         (from_trace extr)
         iatr.
   { eapply (simulation_adequacy_inftraces _ s); eauto.
     eapply from_trace_preserves_validity; eauto; first econstructor.
     simpl. destruct (trfirst extr) eqn:Heq.
     simpl in Hexfirst. rewrite -Hexfirst Heq //. }
-  exists (to_trace (initial_ls (LM := LM) s1 0%nat LSI0) iatr).
+  exists (to_trace (initial_ls' (LM := LM) s1 0%nat LSI0) iatr).
   unshelve eapply (valid_inf_system_trace_implies_traces_match (M := fair_model_model LM_Fair)
             lm_valid_evolution_step
             live_tids
