fairness/fuel_termination.v
@@ -1,6 +1,6 @@
 From stdpp Require Import option.
 From Paco Require Import pacotac.
-From trillium.fairness Require Import fairness fair_termination fuel traces_match lm_fairness_preservation lm_fair lm_fair_traces.
+From trillium.fairness Require Import fairness fair_termination fuel fuel_ext traces_match lm_fairness_preservation lm_fair lm_fair_traces.
 
 Definition auxtrace_fairly_terminating {Λ} {Mdl : FairModel} {LSI}
            {LM : LiveModel (locale Λ) Mdl LSI}
@@ -20,9 +20,10 @@ Theorem continued_simulation_fair_termination
         `{FairTerminatingModel FM} `(LM:LiveModel (locale Λ) FM LSI)
         {LF: LMFairPre LM}
         (ξ : execution_trace Λ → auxiliary_trace (fair_model_model LM_Fair) → Prop) a1 r1 extr
-        (LSI0: let f0 := gset_to_gmap (LM.(lm_fl) a1) (FM.(live_roles) a1) in
-               let m0 := gset_to_gmap r1 (FM.(live_roles) a1) in
-               LSI a1 m0 f0)
+        (* (LSI0: let f0 := gset_to_gmap (LM.(lm_fl) a1) (FM.(live_roles) a1) in *)
+        (*        let m0 := gset_to_gmap r1 (FM.(live_roles) a1) in *)
+        (*        LSI a1 m0 f0) *)
+        (LSI0: initial_ls_LSI a1 r1)
   :
   (* TODO: This is required for destruttering - Not sure why *)
   (∀ c c', locale_step (Λ := Λ) c None c' -> False) →
@@ -33,7 +34,7 @@ Theorem continued_simulation_fair_termination
   (forall (ex: execution_trace Λ) (atr: auxiliary_trace (fair_model_model LM_Fair)),
      ξ ex atr -> lm_valid_state_evolution_fairness ex atr) →
   continued_simulation
-    ξ ({tr[trfirst extr]}) ({tr[initial_ls a1 r1 LSI0]}) →
+    ξ ({tr[trfirst extr]}) ({tr[initial_ls' a1 r1 LSI0]}) →
   extrace_fairly_terminating extr.
 Proof.
   intros Hstep Hlive Hvalid Hsim Hvex.
@@ -42,7 +43,7 @@ Proof.
              valid_inf_system_trace
                (continued_simulation ξ)
                (trace_singleton (trfirst extr))
-               (trace_singleton (initial_ls a1 r1 LSI0))
+               (trace_singleton (initial_ls' a1 r1 LSI0))
                (from_trace extr)
                iatr) as [iatr Hiatr].
   { eexists _. eapply produced_inf_aux_trace_valid_inf. econstructor.
@@ -51,7 +52,7 @@ Proof.
     - eapply from_trace_preserves_validity; eauto; first econstructor. }
   assert (∃ (auxtr : lmftrace), lm_exaux_traces_match extr auxtr)
     as [auxtr Hmatch].
-  { exists (to_trace (initial_ls a1 r1 LSI0) iatr).
+  { exists (to_trace (initial_ls' a1 r1 LSI0) iatr).
     unshelve eapply (valid_inf_system_trace_implies_traces_match
               (lm_valid_evolution_step (LM := LM))
               live_tids
